Parameterize over dereference_scalar in more places
This will allow us to reuse the same code to load inputs and outputs,
when we want to enforce the spec of reading back and removing all of the
values and then saying that the resulting symbolic memory state is
empty.

Some of the proofs are not quite as complete as they were before, but I
hope to replace them soon with a more principled approach.

src/Assembly/EquivalenceProofs.v
@@ -951,8 +951,9 @@ Definition SetRegFresh_G (r : REG) (v : Z) : G.M idx
       G.ret idx)%GM.
 
 Fixpoint build_merge_base_addresses_G
+         {dereference_scalar:bool}
          (items : list (idx + list idx)) (reg_available : list REG) (runtime_reg : list Z) {struct items}
-  : G.M (list (option idx))
+  : G.M (list ((REG + idx) + idx))
   := match items, reg_available, runtime_reg with
      | [], _, _ | _, [], _ => G.ret []
      | _, _, []
@@ -960,21 +961,31 @@ Fixpoint build_merge_base_addresses_G
      | inr idxs :: xs, r :: reg_available, rv :: runtime_reg
        => (base <- SetRegFresh_G r rv; (* note: overwrites initial value *)
            addrs <- G.lift (build_merge_array_addresses base idxs);
-           rest <- build_merge_base_addresses_G xs reg_available runtime_reg;
-           G.ret (Some base :: rest))
+           rest <- build_merge_base_addresses_G (dereference_scalar:=dereference_scalar) xs reg_available runtime_reg;
+           G.ret (inr base :: rest))
      | inl idx :: xs, r :: reg_available, rv :: runtime_reg =>
-          (_ <- G.lift (SetReg r idx); (* note: overwrites initial value *)
-           rest <- build_merge_base_addresses_G xs reg_available runtime_reg;
-           G.ret (None :: rest))
+          (addr <- (if dereference_scalar
+                    then
+                      (addr <- SetRegFresh_G r rv;
+                       G.lift (fun s => Success (inr addr, update_mem_with s (cons (addr, idx)))))
+                    else
+                      (G.lift (_ <- SetReg r idx; (* note: overwrites initial value *)
+                               ret (inl r))));
+           rest <- build_merge_base_addresses_G (dereference_scalar:=dereference_scalar) xs reg_available runtime_reg;
+           G.ret (inl addr :: rest))
      end%GM%N%x86symex.
+
+Definition compute_stack_base_G (rsp_val : Z) (stack_size : nat)
+  : G.M idx
+  := (rsp_idx <- SetRegFresh_G rsp rsp_val;
+      stack_size <- G.lift (Symbolic.App (zconst 64 (-8 * Z.of_nat stack_size), []));
+      G.lift (Symbolic.App (add 64%N, [rsp_idx; stack_size])))%GM.
 
 Definition build_merge_stack_placeholders_G (rsp_val : Z) (stack_vals : list Z)
   : G.M unit
   := (let stack_size := List.length stack_vals in
       stack_placeholders <- lift_dag_G (build_inputarray_G stack_vals);
-      rsp_idx <- SetRegFresh_G rsp rsp_val;
-      stack_size <- G.lift (Symbolic.App (zconst 64 (-8 * Z.of_nat stack_size), []));
-      stack_base <- G.lift (Symbolic.App (add 64%N, [rsp_idx; stack_size]));
+      stack_base <- compute_stack_base_G rsp_val stack_size;
       _ <- G.lift (build_merge_array_addresses stack_base stack_placeholders);
      G.ret tt)%GM.
 
@@ -1423,13 +1434,14 @@ Proof.
                | progress destruct_head'_prod ].
 Qed.
 
-Lemma build_merge_base_addresses_eq_G G items reg_available runtime_reg s res s'
+Lemma build_merge_base_addresses_eq_G {dereference_scalar:bool}
+      G items reg_available runtime_reg s res s'
       (Hreg : Nat.min (List.length items) (List.length reg_available) <= List.length runtime_reg)
-      (H : build_merge_base_addresses items reg_available s = Success (res, s'))
+      (H : build_merge_base_addresses (dereference_scalar:=dereference_scalar) items reg_available s = Success (res, s'))
   : exists G',
-    build_merge_base_addresses_G items reg_available runtime_reg (G, s) = Some (res, (G', s')).
+    build_merge_base_addresses_G (dereference_scalar:=dereference_scalar) items reg_available runtime_reg (G, s) = Some (res, (G', s')).
 Proof.
-  move H at top; move items at top; repeat match goal with H : _ |- _ => revert H end.
+  move H at top; move items at top; move dereference_scalar at top; repeat match goal with H : _ |- _ => revert H end; intro.
   induction items as [|? ? IH]; cbn [build_merge_base_addresses build_merge_base_addresses_G].
   all: cbv [G.ret Symbolic.ret Symbolic.bind ErrorT.bind G.bind Crypto.Util.Option.bind G.lift]; intros.
   all: repeat first [ progress destruct_head'_ex
@@ -1468,6 +1480,32 @@ Proof.
                     | progress destruct_head'_prod ].
 Qed.
 
+Lemma compute_stack_base_eq_G G rsp_val stack_size s res s'
+      (H : compute_stack_base stack_size s = Success (res, s'))
+  : exists G',
+    compute_stack_base_G rsp_val stack_size (G, s) = Some (res, (G', s')).
+Proof.
+  revert H; cbv [compute_stack_base_G compute_stack_base G.bind G.ret Crypto.Util.Option.bind Symbolic.bind ErrorT.bind G.lift Symbolic.ret].
+  repeat first [ progress intros
+               | progress cbn [fst snd] in *
+               | progress subst
+               | progress inversion_ErrorT
+               | progress inversion_option
+               | progress destruct_head'_prod
+               | progress subst_prod
+               | progress destruct_head'_ex
+               | eexists; reflexivity
+               | match goal with
+                 | [ H : SetRegFresh _ _ = Success _ |- _ ]
+                   => eapply SetRegFresh_eq_G in H
+                 | [ H : SetRegFresh_G ?r ?v ?s = _, H' : SetRegFresh_G ?r' ?v' ?s' = _ |- _ ]
+                   => unify r r'; unify v v'; unify s s'; rewrite H in H'
+                 | [ H : ?x = Success _ |- context[?x] ] => rewrite H
+                 end
+               | break_innermost_match_hyps_step
+               | break_innermost_match_step ].
+Qed.
+
 Lemma build_merge_stack_placeholders_eq_G G rsp_val stack_vals s res s'
       (H : build_merge_stack_placeholders (List.length stack_vals) s = Success (res, s'))
   : exists G',
@@ -1484,9 +1522,9 @@ Proof.
                | progress destruct_head'_ex
                | eexists; reflexivity
                | match goal with
-                 | [ H : SetRegFresh _ _ = Success _ |- _ ]
-                   => eapply SetRegFresh_eq_G in H
-                 | [ H : SetRegFresh_G ?r ?v ?s = _, H' : SetRegFresh_G ?r' ?v' ?s' = _ |- _ ]
+                 | [ H : compute_stack_base _ _ = Success _ |- _ ]
+                   => eapply compute_stack_base_eq_G in H
+                 | [ H : compute_stack_base_G ?r ?v ?s = _, H' : compute_stack_base_G ?r' ?v' ?s' = _ |- _ ]
                    => unify r r'; unify v v'; unify s s'; rewrite H in H'
                  | [ H : lift_dag _ _ = Success _ |- _ ]
                    => eapply lift_dag_eq_G in H; [ | clear H ]
@@ -2109,6 +2147,80 @@ Proof.
   reflexivity.
 Qed.
 
+Lemma compute_stack_base_G_ok G G' s s' rv
+      (rsp_val : Z) (stack_size : nat)
+      (H : compute_stack_base_G rsp_val stack_size (G, s) = Some (rv, (G', s')))
+      (d := s.(dag_state))
+      (d' := s'.(dag_state))
+      (r := s.(symbolic_reg_state))
+      (r' := s'.(symbolic_reg_state))
+      (f := s.(symbolic_flag_state))
+      (f' := s'.(symbolic_flag_state))
+      (m := s.(symbolic_mem_state))
+      (m' := s'.(symbolic_mem_state))
+      (Hd : gensym_dag_ok G d)
+  : ((exists rsp_idx,
+         set_reg r (reg_index rsp) rsp_idx = r'
+         /\ eval_idx_Z G' d' rsp_idx (Z.land rsp_val (Z.ones 64)))
+     /\ f = f'
+     /\ m = m')
+    /\ eval_idx_Z G' d' rv (Z.land (rsp_val - 8 * Z.of_nat stack_size) (Z.ones 64))
+    /\ gensym_dag_ok G' d'
+    /\ (forall e n, eval G d e n -> eval G' d' e n).
+Proof.
+  cbv [compute_stack_base_G ret Symbolic.bind ErrorT.bind G.bind G.lift Crypto.Util.Option.bind lift_dag_G G.ret] in H.
+  break_match_hyps.
+  all: repeat first [ progress inversion_option
+                    | progress inversion_ErrorT
+                    | progress subst
+                    | progress destruct_head'_and
+                    | progress destruct_head'_prod
+                    | progress cbn [fst snd dag_state update_dag_with update_mem_with symbolic_reg_state symbolic_flag_state] in *
+                    | progress destruct_head'_prod
+                    | progress destruct_head'_ex
+                    | assumption
+                    | progress intros
+                    | solve [ eauto ]
+                    | progress break_innermost_match_hyps
+                    | rewrite @fold_left_id in *
+                    | progress cbv [Symbolic.App Merge] in *
+                    | progress cbn [fold_right update_dag_with Symbolic.dag_state Symbolic.symbolic_mem_state] in *
+                    | progress change (Z.of_N 64) with 64%Z in *
+                    | match goal with
+                      | [ H : (?x, ?y) = (?x', ?y') |- _ ]
+                        => first [ is_var x | is_var y ]; is_var x'; is_var y'; inversion H; clear H
+                      | [ H : (?x, (?y, ?z)) = (?x', (?y', ?z')) |- _ ]
+                        => is_var x; is_var y; is_var x'; is_var y'; is_var z'; inversion H; clear H
+                      | [ H : (tt, (?y, ?z)) = (tt, (?y', ?z')) |- _ ]
+                        => is_var y; is_var z; is_var y'; is_var z'; inversion H; clear H
+                      | [ H : context[simplify ?s ?n] |- _ ]
+                        => unshelve epose proof (@eval_simplify _ s n _ _); shelve_unifiable;
+                           [ solve [ repeat first [ eassumption | solve [ eauto ] | exactly_once econstructor ] ] | ];
+                           generalize dependent (simplify s n); intros
+                      | [ H : context[merge ?e ?d] |- _ ]
+                        => pose proof (@eval_merge _ e _ d ltac:(eassumption) ltac:(eassumption));
+                           generalize dependent (merge e d); intros
+                      | [ H : SetRegFresh_G _ _ _ = _ |- _ ]
+                        => eapply SetRegFresh_G_ok in H;
+                           [
+                           | lazymatch goal with
+                             | [ |- index_and_shift_and_bitcount_of_reg _ = _ ] => cbv; reflexivity
+                             | _ => idtac
+                             end .. ];
+                           [ | solve [ reflexivity | assumption | split; assumption ] .. ]
+                      | [ H : eval ?G ?d ?i ?v |- eval ?G ?d ?i ?v' ]
+                        => replace v' with v; [ exact H | ]
+                      | [ H := _ |- _ ] => subst H
+                      end
+                    | progress cbn [Symbolic.dag_state Symbolic.symbolic_reg_state Symbolic.symbolic_mem_state Symbolic.symbolic_flag_state] in *
+                    | progress destruct_head' symbolic_state
+                    | progress cbv [eval_idx_Z] in *
+                    | apply conj; eauto 10; []
+                    | rewrite !Z.land_ones in * by lia
+                    | progress (push_Zmod; pull_Zmod)
+                    | f_equal; lia ].
+Qed.
+
 Lemma build_merge_stack_placeholders_G_ok G G' s s'
       (rsp_val : Z) (stack_vals : list Z)
       (H : build_merge_stack_placeholders_G rsp_val stack_vals (G, s) = Some (tt, (G', s')))
@@ -2159,26 +2271,14 @@ Proof.
                         => is_var x; is_var y; is_var x'; is_var y'; is_var z'; inversion H; clear H
                       | [ H : (tt, (?y, ?z)) = (tt, (?y', ?z')) |- _ ]
                         => is_var y; is_var z; is_var y'; is_var z'; inversion H; clear H
-                      | [ H : context[simplify ?s ?n] |- _ ]
-                        => unshelve epose proof (@eval_simplify _ s n _ _); shelve_unifiable;
-                           [ solve [ repeat first [ eassumption | solve [ eauto ] | exactly_once econstructor ] ] | ];
-                           generalize dependent (simplify s n); intros
-                      | [ H : context[merge ?e ?d] |- _ ]
-                        => pose proof (@eval_merge _ e _ d ltac:(eassumption) ltac:(eassumption));
-                           generalize dependent (merge e d); intros
-                      | [ H : SetRegFresh_G _ _ _ = _ |- _ ]
-                        => eapply SetRegFresh_G_ok in H;
-                           [
-                           | lazymatch goal with
-                             | [ |- index_and_shift_and_bitcount_of_reg _ = _ ] => cbv; reflexivity
-                             | _ => idtac
-                             end .. ];
-                           [ | solve [ reflexivity | assumption | split; assumption ] .. ]
+                      | [ H : compute_stack_base_G _ _ _ = _ |- _ ]
+                        => eapply compute_stack_base_G_ok in H;
+                           [ | assumption ]
                       | [ H : build_inputarray_G _ _ = _ |- _ ]
                         => apply build_inputarray_G_ok in H; [ | assumption .. ]
                       | [ H : build_merge_array_addresses _ _ _ = _ |- _ ]
                         => eapply build_merge_array_addresses_ok in H;
-                           [ | try solve [ assumption | lia ] .. ]
+                           [ | clear H; try solve [ assumption | lia ] .. ]
                       | [ H := _ |- _ ] => subst H
                       end ].
   { cbv [eval_idx_Z update_mem_with symbolic_reg_state dag_state symbolic_mem_state symbolic_flag_state update_dag_with reg_index] in *; destruct_head' symbolic_state; subst.
@@ -2204,16 +2304,19 @@ Proof.
 Qed.
 
 Lemma build_merge_base_addresses_G_ok
+      {dereference_scalar:bool}
   : forall (idxs : list (idx + list idx))
            (reg_available : list REG)
            (runtime_reg : list Z)
            G s G' s'
            outputaddrs
-           (H : build_merge_base_addresses_G idxs reg_available runtime_reg (G, s) = Some (outputaddrs, (G', s')))
+           (H : build_merge_base_addresses_G (dereference_scalar:=dereference_scalar) idxs reg_available runtime_reg (G, s) = Some (outputaddrs, (G', s')))
            (d := s.(dag_state))
            (Hvals : Forall2 (fun it rv
                              => match it with
-                                | inl idx => eval_idx_Z G d idx rv
+                                | inl idx => if dereference_scalar
+                                             then True
+                                             else eval_idx_Z G d idx rv
                                 | inr _ => True
                                 end)
                             idxs (List.firstn (List.length idxs) runtime_reg))
@@ -2228,12 +2331,12 @@ Lemma build_merge_base_addresses_G_ok
            (m' := s'.(symbolic_mem_state))
            (Hd : gensym_dag_ok G d)
            (Hreg_available_wide : Forall (fun reg => let '(rn, lo, sz) := index_and_shift_and_bitcount_of_reg reg in sz = 64%N) reg_available),
-    ((exists (outputaddrs' : list (idx + idx * list idx)),
+    ((exists (outputaddrs' : list (idx * option idx + idx * list idx)),
          let addrs_vals_of := fun base_reg_val addrs' => List.map (fun i => Z.land (base_reg_val + 8 * Z.of_nat i) (Z.ones 64)) (seq 0 (List.length addrs')) in
          fold_left (fun rst '(r, idx')
                     => set_reg rst (reg_index r)
                                match idx' with
-                               | inl idx' => idx'
+                               | inl (idx', _) => idx'
                                | inr (base_idx', idxs') => base_idx'
                                end)
                    (List.combine reg_available outputaddrs')
@@ -2243,7 +2346,8 @@ Lemma build_merge_base_addresses_G_ok
              List.rev (List.flat_map
                          (fun '(idx', idx)
                           => match idx', idx with
-                             | inl _, inl _ => []
+                             | inl (reg_val, Some addr), inl val => if dereference_scalar then [(addr, val)] else []
+
                              | inl _, _ | _, inl _ => []
                              | inr (base', addrs'), inr items
                                => List.combine addrs' items
@@ -2255,8 +2359,9 @@ Lemma build_merge_base_addresses_G_ok
            Forall2
              (fun idx' v =>
                 match idx' with
-                | inl idx' (* scalars *)
+                | inl (idx', addr') (* scalars *)
                   => eval_idx_Z G' d' idx' (Z.land v (Z.ones 64))
+                     /\ option_eq (eval_idx_Z G' d') addr' (if dereference_scalar then Some (Z.land v (Z.ones 64)) else None)
                 | inr (base', addrs')
                   (* arrays: (exists base',
                     (* set_reg r rn base' = r'
@@ -2272,11 +2377,21 @@ Lemma build_merge_base_addresses_G_ok
            Forall2
              (fun idx base_reg_val =>
                 match idx with
-                | Some base => eval_idx_Z G' d' base (Z.land base_reg_val (Z.ones 64))
-                | None => True
+                | inr base => eval_idx_Z G' d' base (Z.land base_reg_val (Z.ones 64))
+                | inl (inr base) => eval_idx_Z G' d' base (Z.land base_reg_val (Z.ones 64))
+                | inl (inl r) => True
                 end)
              outputaddrs
              (List.firstn (List.length outputaddrs) runtime_reg)
+         /\ (* outputaddrs reg: *)
+           Forall2
+             (fun idx r =>
+                match idx with
+                | inl (inl r') => r = r'
+                | inl (inr _) | inr _ => True
+                end)
+             outputaddrs
+             (List.firstn (List.length outputaddrs) reg_available)
          /\ Forall2 (fun addr idx =>
                        match addr, idx with
                        | inl _, inl _ => True
@@ -2286,9 +2401,9 @@ Lemma build_merge_base_addresses_G_ok
                     outputaddrs' idxs
          /\ Forall2 (fun addr idx =>
                        match addr, idx with
-                       | None, inl _ => True
-                       | Some _, inr _ => True
-                       | None, inr _ | Some _, inl _ => False
+                       | inl _, inl (_, addr) => Option.is_Some addr = dereference_scalar
+                       | inr _, inr _ => True
+                       | inl _, inr _ | inr _, inl _ => False
                        end)
                     outputaddrs outputaddrs')
      /\ f = f')
@@ -2300,7 +2415,7 @@ Proof.
         runtime_reg as [|runtime_reg runtime_regs];
     try specialize (IH reg_availables runtime_regs).
   all: repeat first [ progress cbn [build_merge_base_addresses_G List.length firstn] in *
-                    | progress cbv [G.ret G.lift G.bind Crypto.Util.Option.bind] in *
+                    | progress cbv [Symbolic.bind ErrorT.bind Symbolic.ret G.ret G.lift G.bind Crypto.Util.Option.bind] in *
                     | progress intros
                     | progress inversion_option
                     | progress inversion_prod
@@ -2319,7 +2434,7 @@ Proof.
                | assumption
                | progress specialize_by_assumption
                | progress specialize_by (eapply Forall2_weaken; [ | eassumption ]; intros; break_innermost_match; eauto using lift_eval_idx_Z_impl)
-               | progress cbn [length firstn List.combine fold_left flat_map rev Symbolic.dag_state Symbolic.symbolic_reg_state Symbolic.symbolic_mem_state Symbolic.symbolic_flag_state] in *
+               | progress cbn [length firstn List.combine fold_left flat_map rev Symbolic.dag_state Symbolic.symbolic_reg_state Symbolic.symbolic_mem_state Symbolic.symbolic_flag_state update_mem_with fst snd] in *
                | progress destruct_head' symbolic_state
                | match goal with
                  | [ H : (_, _) = (_, _) |- _ ] => inversion H; clear H
@@ -2348,18 +2463,30 @@ Proof.
                         => is_var x; destruct x*)
                  end
                | break_innermost_match_hyps_step
-               | apply conj; eauto 10; [] ].
+               | apply conj; eauto 10; []
+               | progress cbv [index_and_shift_and_bitcount_of_reg] in * ].
   (* above is all reversible, evar-free; below is irreversible *)
-  all: [ > eexists (inl _ :: _) | eexists (inr (_, _) :: _) ].
+  all: exactly_once ((lazymatch goal with |- context[inr _ :: _] => idtac end;
+                      eexists (inr (_, _) :: _))
+                     + (lazymatch goal with |- context[inl (inl _) :: _] => idtac end;
+                        eexists (inl (_, None) :: _))
+                     + (lazymatch goal with |- context[inl (inr _) :: _] => idtac end;
+                        eexists (inl (_, Some _) :: _))).
   all: repeat
          repeat
-         first [ rewrite rev_app_distr
+         first [ progress cbn [length firstn List.combine fold_left flat_map rev] in *
+               | rewrite rev_app_distr
+               | rewrite <- ?app_assoc; progress cbn [List.app]
                | rewrite !app_assoc
                | rewrite app_nil_r
-               | progress cbv [index_and_shift_and_bitcount_of_reg] in *
-               | progress cbn [length firstn List.combine fold_left flat_map rev] in *
+               | progress cbv [option_eq] in *
                | progress inversion_prod
                | progress subst
+               | (* instantiate evars early to avoid wrong instantiations *)
+                 match goal with
+                 | [ |- context[?x ++ ?y :: ?z = ?x' ++ ?y' :: ?z] ]
+                   => progress unify y y'
+                 end
                | reflexivity
                | eassumption
                | solve [ eauto using Forall2_weaken, lift_eval_idx_Z_impl ]
@@ -2367,6 +2494,8 @@ Proof.
                | match goal with
                  | [ |- Forall2 _ (_ :: _) (_ :: _) ] => constructor
                  | [ |- fold_left ?f _ _ = fold_left ?f _ _ ] => f_equal
+                 | [ |- _ :: _ = _ :: _ ] => f_equal
+                 | [ |- (_, _) = (_, _) ] => f_equal
                  | [ |- ?x ++ ?y = ?x' ++ ?y ] => f_equal
                  | [ |- ?x ++ ?y = ?x ++ ?y' ] => f_equal
                  | [ |- rev _ = rev _ ] => apply f_equal
@@ -2385,6 +2514,33 @@ Proof.
                       [ eauto using lift_eval_idx_Z_impl
                       | intros; rewrite !Z.land_ones by lia; push_Zmod; pull_Zmod ]
                  end ].
+Qed.
+
+Lemma compute_stack_ok G s s' base
+      (rsp_val : Z) (stack_size : nat)
+      (H : compute_stack_base stack_size s = Success (base, s'))
+      (d := s.(dag_state))
+      (d' := s'.(dag_state))
+      (r := s.(symbolic_reg_state))
+      (r' := s'.(symbolic_reg_state))
+      (f := s.(symbolic_flag_state))
+      (f' := s'.(symbolic_flag_state))
+      (m := s.(symbolic_mem_state))
+      (m' := s'.(symbolic_mem_state))
+      (Hd : gensym_dag_ok G d)
+  : exists G',
+    ((exists rsp_idx,
+         set_reg r (reg_index rsp) rsp_idx = r'
+         /\ eval_idx_Z G' d' rsp_idx (Z.land rsp_val (Z.ones 64)))
+     /\ f = f'
+     /\ m = m')
+    /\ eval_idx_Z G' d' base (Z.land (rsp_val - 8 * Z.of_nat stack_size) (Z.ones 64))
+    /\ gensym_dag_ok G' d'
+    /\ (forall e n, eval G d e n -> eval G' d' e n).
+Proof.
+  eapply compute_stack_base_eq_G in H.
+  destruct H as [G' H]; exists G'.
+  eapply compute_stack_base_G_ok in H; try eassumption.
 Qed.
 
 Lemma build_merge_stack_placeholders_ok G s s'
@@ -2419,6 +2575,7 @@ Proof.
 Qed.
 
 Lemma build_merge_base_addresses_ok
+      {dereference_scalar:bool}
       (idxs : list (idx + list idx))
       (reg_available : list REG)
       (runtime_reg : list Z)
@@ -2426,7 +2583,9 @@ Lemma build_merge_base_addresses_ok
       (d := s.(dag_state))
       (Hvals : Forall2 (fun it rv
                         => match it with
-                           | inl idx => eval_idx_Z G d idx rv
+                           | inl idx => if dereference_scalar
+                                        then True
+                                        else eval_idx_Z G d idx rv
                            | inr _ => True
                            end)
                        idxs (List.firstn (List.length idxs) runtime_reg))
@@ -2441,16 +2600,16 @@ Lemma build_merge_base_addresses_ok
       (m := s.(symbolic_mem_state))
       (m' := s'.(symbolic_mem_state))
       outputaddrs
-      (H : build_merge_base_addresses idxs reg_available s = Success (outputaddrs, s'))
+      (H : build_merge_base_addresses (dereference_scalar:=dereference_scalar) idxs reg_available s = Success (outputaddrs, s'))
       (Hd : gensym_dag_ok G d)
       (Hreg_available_wide : Forall (fun reg => let '(rn, lo, sz) := index_and_shift_and_bitcount_of_reg reg in sz = 64%N) reg_available)
   : exists G',
-    ((exists (outputaddrs' : list (idx + idx * list idx)),
+    ((exists (outputaddrs' : list (idx * option idx + idx * list idx)),
          let addrs_vals_of := fun base_reg_val addrs' => List.map (fun i => Z.land (base_reg_val + 8 * Z.of_nat i) (Z.ones 64)) (seq 0 (List.length addrs')) in
          fold_left (fun rst '(r, idx')
                     => set_reg rst (reg_index r)
                                match idx' with
-                               | inl idx' => idx'
+                               | inl (idx', _) => idx'
                                | inr (base_idx', idxs') => base_idx'
                                end)
                    (List.combine reg_available outputaddrs')
@@ -2460,7 +2619,8 @@ Lemma build_merge_base_addresses_ok
              List.rev (List.flat_map
                          (fun '(idx', idx)
                           => match idx', idx with
-                             | inl _, inl _ => []
+                             | inl (reg_val, Some addr), inl val => if dereference_scalar then [(addr, val)] else []
+
                              | inl _, _ | _, inl _ => []
                              | inr (base', addrs'), inr items
                                => List.combine addrs' items
@@ -2472,8 +2632,9 @@ Lemma build_merge_base_addresses_ok
            Forall2
              (fun idx' v =>
                 match idx' with
-                | inl idx' (* scalars *)
+                | inl (idx', addr') (* scalars *)
                   => eval_idx_Z G' d' idx' (Z.land v (Z.ones 64))
+                     /\ option_eq (eval_idx_Z G' d') addr' (if dereference_scalar then Some (Z.land v (Z.ones 64)) else None)
                 | inr (base', addrs')
                   (* arrays: (exists base',
                     (* set_reg r rn base' = r'
@@ -2489,11 +2650,21 @@ Lemma build_merge_base_addresses_ok
            Forall2
              (fun idx base_reg_val =>
                 match idx with
-                | Some base => eval_idx_Z G' d' base (Z.land base_reg_val (Z.ones 64))
-                | None => True
+                | inr base => eval_idx_Z G' d' base (Z.land base_reg_val (Z.ones 64))
+                | inl (inr base) => eval_idx_Z G' d' base (Z.land base_reg_val (Z.ones 64))
+                | inl (inl r) => True
                 end)
              outputaddrs
              (List.firstn (List.length outputaddrs) runtime_reg)
+         /\ (* outputaddrs reg: *)
+           Forall2
+             (fun idx r =>
+                match idx with
+                | inl (inl r') => r = r'
+                | inl (inr _) | inr _ => True
+                end)
+             outputaddrs
+             (List.firstn (List.length outputaddrs) reg_available)
          /\ Forall2 (fun addr idx =>
                        match addr, idx with
                        | inl _, inl _ => True
@@ -2503,9 +2674,9 @@ Lemma build_merge_base_addresses_ok
                     outputaddrs' idxs
          /\ Forall2 (fun addr idx =>
                        match addr, idx with
-                       | None, inl _ => True
-                       | Some _, inr _ => True
-                       | None, inr _ | Some _, inl _ => False
+                       | inl _, inl (_, addr) => Option.is_Some addr = dereference_scalar
+                       | inr _, inr _ => True
+                       | inl _, inr _ | inr _, inl _ => False
                        end)
                     outputaddrs outputaddrs')
      /\ f = f')
@@ -2515,6 +2686,28 @@ Proof.
   eapply build_merge_base_addresses_eq_G in H; [ | eassumption .. ].
   destruct H as [G' H]; exists G'.
   eapply build_merge_base_addresses_G_ok in H; try eassumption.
+Qed.
+
+Lemma Load64_ok G s s' addr addr_val idx
+      (H : Load64 addr s = Success (idx, s'))
+      (d := s.(dag_state))
+      (d' := s'.(dag_state))
+      (r := s.(symbolic_reg_state))
+      (r' := s'.(symbolic_reg_state))
+      (f := s.(symbolic_flag_state))
+      (f' := s'.(symbolic_flag_state))
+      (m := s.(symbolic_mem_state))
+      (m' := s'.(symbolic_mem_state))
+      (Hd : gensym_dag_ok G d)
+      (Haddr : eval_idx_Z G d addr addr_val)
+  : (Some idx = load addr s'
+     /\ r = r'
+     /\ f = f'
+     /\ m = m')
+    /\ gensym_dag_ok G d'
+    /\ (forall e n, eval G d e n -> eval G d' e n).
+Proof.
+  cbv [Load64 some_or] in *; break_innermost_match_hyps; inversion_ErrorT; inversion_pair; subst; intuition eauto.
 Qed.
 
 Lemma LoadArray_ok G s s' base base_val len idxs
@@ -2578,8 +2771,8 @@ Proof.
                     | solve [ eauto using lift_eval_idx_Z_impl ] ].
 Qed.
 
-Lemma LoadOutputs_ok G s s' outputaddrs output_types output_vals idxs
-      (H : LoadOutputs outputaddrs output_types s = Success (idxs, s'))
+Lemma LoadOutputs_ok {dereference_scalar:bool} G s s' outputaddrs output_types output_vals idxs
+      (H : LoadOutputs (dereference_scalar:=dereference_scalar) outputaddrs output_types s = Success (idxs, s'))
       (d := s.(dag_state))
       (d' := s'.(dag_state))
       (r := s.(symbolic_reg_state))
@@ -2589,16 +2782,29 @@ Lemma LoadOutputs_ok G s s' outputaddrs output_types output_vals idxs
       (m := s.(symbolic_mem_state))
       (m' := s'.(symbolic_mem_state))
       (Hd : gensym_dag_ok G d)
-      (Houtputaddrs : Forall2 (fun idx val
-                               => match idx with
-                                  | Some idx => eval_idx_Z G d idx (Z.land val (Z.ones 64))
-                                  | _ => True
-                                  end) outputaddrs output_vals)
+      (Houtputaddrs_array : Forall2 (fun idx val
+                                     => match idx with
+                                        | inr idx => eval_idx_Z G d idx (Z.land val (Z.ones 64))
+                                        | _ => True
+                                        end) outputaddrs output_vals)
+      (Houtputaddrs_reg : Forall (fun idx
+                                  => match idx with
+                                     | inl (inl r)
+                                       => (let '(rn, lo, sz) := index_and_shift_and_bitcount_of_reg r in sz = 64%N)
+                                            /\ (exists v, forall idx', get_reg s (reg_index r) = Some idx' -> eval_idx_Z G s idx' (Z.land v (Z.ones 64)))
+                                     | _ => True
+                                     end) outputaddrs)
   : ((exists outputaddrs' : list (idx + list idx),
          Forall2 (fun idxs '((base, len), base_val)
                   => match idxs, base, len with
-                     | inr idxs, Some base, Some len
+                     | inr idxs, inr base, Some len
                        => Forall2 (eval_idx_Z G d') idxs (List.map (fun i => Z.land (base_val + 8 * Z.of_nat i) (Z.ones 64)) (seq 0 len))
+                     | inl idx, inl (inl r), None
+                       => (exists idx',
+                              get_reg s' (reg_index r) = Some idx'
+                              /\ forall v, eval_idx_Z G d' idx v -> eval_idx_Z G d' idx' v)
+                     | inl idx, inl (inr addr), None
+                       => idx = addr
                      | _, _, _ => False
                      end)
                  outputaddrs'
@@ -2608,7 +2814,9 @@ Lemma LoadOutputs_ok G s s' outputaddrs output_types output_vals idxs
                 (List.map (fun idxs
                            => match idxs with
                               | inr idxs => option_map inr (Option.List.lift (List.map (fun a => load a s') idxs))
-                              | inl idx => None (* Some (inl idx) ?? *)
+                              | inl idx => if dereference_scalar
+                                           then option_map inl (load idx s')
+                                           else Some (inl idx)
                               end)
                           outputaddrs'))
      /\ r = r'
@@ -2618,28 +2826,27 @@ Lemma LoadOutputs_ok G s s' outputaddrs output_types output_vals idxs
     /\ (forall e n, eval G d e n -> eval G d' e n).
 Proof.
   cbv [LoadOutputs Symbolic.bind Symbolic.ret ErrorT.bind] in H.
-  break_match_hyps.
-  all: repeat first [ progress inversion_ErrorT
-                    | progress inversion_prod
-                    | progress subst
-                    | progress destruct_head'_prod
-                    | progress cbn [fst snd] in *
-                    | match goal with
-                      | [ H := _ |- _ ] => subst H
-                      end ].
+  repeat first [ progress inversion_ErrorT
+               | progress inversion_prod
+               | progress subst
+               | progress destruct_head'_prod
+               | progress cbn [fst snd] in *
+               | match goal with
+                 | [ H := _ |- _ ] => subst H
+                 end ].
   match goal with
   | [ H : mapM _ _ _ = Success (?l, ?s) |- _ ]
     => rename l into idxs; rename s into s'
   end.
-  revert Houtputaddrs.
-  revert Hd.
+  revert Hd Houtputaddrs_array Houtputaddrs_reg.
   revert dependent s'.
   revert outputaddrs output_types output_vals idxs s.
   induction outputaddrs as [|outputaddr outputaddrs IH],
       output_types as [|output_type output_types],
         output_vals as [|output_val output_vals],
-          idxs as [|idx idxs];
+            idxs as [|idx idxs];
     try specialize (IH output_types output_vals idxs).
+  all: intros; repeat match goal with |- _ /\ _ => apply conj end.
   all: repeat first [ progress cbn [fst snd mapM List.map List.combine option_map fold_right Crypto.Util.Option.bind Symbolic.dag_state Symbolic.symbolic_reg_state Symbolic.symbolic_mem_state Symbolic.symbolic_flag_state] in *
                     | progress cbv [Symbolic.ret] in *
                     | progress intros
@@ -2653,6 +2860,7 @@ Proof.
                     | progress destruct_head'_and
                     | progress specialize_by_assumption
                     | match goal with
+                      | [ H : Forall _ (_ :: _) |- _ ] => inversion H; clear H
                       | [ H : Forall2 _ (_ :: _) _ |- _ ] => inversion H; clear H
                       | [ H : Forall2 _ [] _ |- _ ] => inversion H; clear H
                       | [ H : _ :: _ = _ :: _ |- _ ] => inversion H; clear H
@@ -2663,6 +2871,8 @@ Proof.
                         => is_var x; destruct x
                       | [ H : LoadArray _ _ _ = _ |- _ ]
                         => eapply LoadArray_ok in H; [ | eassumption .. ]
+                      | [ H : GetReg _ _ = _ |- _ ]
+                        => eapply GetReg_ok in H; [ | (reflexivity + eassumption) .. ]
                       | [ H : Some _ = _ |- _ ] => rewrite <- H
                       | [ |- Forall2 _ (_ :: _) (_ :: _) ] => constructor
                       | [ H : Forall2 _ ?ls (List.map ?f ?ls') |- Forall2 _ ?ls (List.map ?f' ?ls') ]
@@ -2670,14 +2880,37 @@ Proof.
                            cbv beta;
                            [ solve [ eauto using lift_eval_idx_Z_impl ]
                            | intros; rewrite !Z.land_ones by lia; push_Zmod; try reflexivity ]
+                      | [ H : load _ _ = Some _ |- context[load] ] => rewrite H
+                      | [ H : ?v = Some _ |- exists x, ?v = Some x /\ _ ] => eexists; split; eauto
+                      | [ H : eval_idx_Z _ _ ?i ?v, H' : eval_idx_Z _ _ ?i ?v' |- _ ]
+                        => eapply eval_eval_idx_Z in H'; [ | eapply lift_eval_idx_Z_impl; [ | exact H ]; now eauto ]
                       end
-                    | progress cbv [Symbolic.bind ErrorT.bind] in *
+                    | rewrite Z.land_same_r in *
+                    | progress cbv [Symbolic.bind ErrorT.bind Load64 some_or option_map] in *
                     | break_innermost_match_hyps_step
                     | progress break_match_hyps
-                    | progress specialize_by (eapply Forall2_weaken; [ | eassumption ]; cbv beta; intros *; break_innermost_match; eauto using lift_eval_idx_Z_impl)
-                    | apply conj; eauto; []
-                    | eexists (inr _ :: _)
-                    | progress cbv [Option.List.lift] in * ].
+                    | progress specialize_by
+                               (first [ eapply Forall2_weaken | eapply Forall_impl ]; [ | multimatch goal with H : _ |- _ => exact H end ];
+                                cbv beta; intros *;
+                                destruct_head' symbolic_state; cbn [Symbolic.dag_state Symbolic.symbolic_reg_state Symbolic.symbolic_mem_state Symbolic.symbolic_flag_state] in *;
+                                subst;
+                                break_innermost_match;
+                                cbv [eval_idx_Z] in *;
+                                now intuition (destruct_head'_ex; eauto))
+                    | apply conj;
+                      match goal with
+                      | [ |- ?G ] => tryif has_evar G then auto else eauto
+                      end;
+                      []
+                    | progress destruct_head' symbolic_state
+                    | match goal with
+                      | [ |- context[Forall2 _ _ ((inr _, _, _) :: _)] ]
+                        => eexists (inr _ :: _)
+                      | [ |- context[Forall2 _ _ ((inl _, _, _) :: _)] ]
+                        => eexists (inl _ :: _)
+                      end
+                    | progress cbv [Option.List.lift] in *
+                    | solve [ eauto using lift_eval_idx_Z_impl ] ].
 Qed.
 
 Lemma mapM_GetReg_ok_bounded G
